transformations/Moore2MealyALT/theorems/Elements.v
@@ -13,19 +13,20 @@ Variable (m:Moore.M).
 Hypothesis WF_U : MooreWF.unique_ids m.
 Hypothesis WF_T : Moore.WF_target m.
 
-Definition convert (s:Moore.State_t) : Mealy.State_t :=
+Definition convert_state (s:Moore.State_t) : Mealy.State_t :=
   {| Mealy.State_id := s.(Moore.State_id) |}.
 
-Lemma convert_injective : 
+(** [convert_state] is not injective, but if we consider states of a model with uniqueness of identifiers, it becomes injective. *)
+Lemma convert_state_injective : 
   forall s1 s2,
     List.In (Moore.StateElement s1) m.(Model.modelElements) ->
     List.In (Moore.StateElement s2) m.(Model.modelElements) ->
-    convert s1 = convert s2 ->
+    convert_state s1 = convert_state s2 ->
     s1 = s2.
 Proof.
   intros s1 s2 H1 H2 H3.
   apply WF_U ; auto.
-  destruct s1, s2 ; unfold convert in H3 ; congruence.
+  destruct s1, s2 ; unfold convert_state in H3 ; congruence.
 Qed.
 
 
@@ -38,7 +39,7 @@ Definition convert_transition  (t : Moore.Transition_t)   :option Mealy.Transiti
 
 Lemma convert_transition_injective : 
   forall t1 t2 a, 
-    convert_transition t1 = Some a -> (* would be false with None *)
+    convert_transition t1 = Some a -> 
     convert_transition t2 = Some a ->
     t1 = t2.
 Proof.
@@ -49,8 +50,8 @@ Proof.
   destruct t1, t2 ; simpl in * ; congruence.
 Qed.
 
-
-Lemma convert_transition_ok : forall t,
+(* not used *)
+Lemma convert_transition_suff : forall t,
     List.In (Moore.TransitionElement t) m.(Model.modelElements) -> 
     SUCCESS (convert_transition t).
 Proof.
@@ -65,8 +66,14 @@ Qed.
 
 Lemma convert_transition_ok2 : forall t,
     List.In (Moore.TransitionElement t) m.(Model.modelElements) -> 
-    exists s, Moore.getTransition_target m t = Some s /\
-    convert_transition t = Some (Mealy.Build_Transition_t t.(Moore.Transition_source) t.(Moore.Transition_input) s.(Moore.State_output) t.(Moore.Transition_dest)).
+    exists s,
+      Moore.getTransition_target m t = Some s /\
+        convert_transition t = 
+          Some (Mealy.Build_Transition_t 
+                  t.(Moore.Transition_source) 
+                      t.(Moore.Transition_input) 
+                          s.(Moore.State_output) 
+                              t.(Moore.Transition_dest)).
 Proof.
   intros t H.
   apply WF_T in H.
@@ -78,14 +85,15 @@ Proof.
   reflexivity.
 Qed.  
 
-Lemma convert_transition_inv t t':
+Lemma convert_transition_nec t t':
   convert_transition t = Some t' ->
   exists s,
-  Moore.getTransition_target m t = Some s /\ t' ={|
-    Mealy.Transition_source := Moore.Transition_source t;
-    Mealy.Transition_input := Moore.Transition_input t;
-    Mealy.Transition_output := Moore.State_output s;
-    Mealy.Transition_dest := Moore.Transition_dest t
+  Moore.getTransition_target m t = Some s /\ 
+    t' ={|
+     Mealy.Transition_source := Moore.Transition_source t;
+     Mealy.Transition_input := Moore.Transition_input t;
+     Mealy.Transition_output := Moore.State_output s;
+     Mealy.Transition_dest := Moore.Transition_dest t
   |}.
 Proof.    
   unfold convert_transition ; intro.
@@ -99,7 +107,7 @@ Notation transform_element_fw :=
 Lemma state_element_fw : 
   forall (s:Moore.State_t),
     List.In (Moore.StateElement s) (Model.modelElements m) ->
-    List.In (Mealy.StateElement (convert s))  (Semantics.execute  Moore2Mealy.Moore2Mealy m).(Model.modelElements).
+    List.In (Mealy.StateElement (convert_state s))  (Semantics.execute  Moore2Mealy.Moore2Mealy m).(Model.modelElements).
 Proof.
   intros s IN.
   eapply transform_element_fw ; eauto. 
@@ -110,7 +118,7 @@ Lemma state_element_bw :
   forall (s:Mealy.State_t),
     List.In (Mealy.StateElement s) (Model.modelElements (Semantics.execute  Moore2Mealy.Moore2Mealy m)) ->
     exists s0,
-      List.In (Moore.StateElement s0) (Model.modelElements m) /\ s = convert s0.
+      List.In (Moore.StateElement s0) (Model.modelElements m) /\ s = convert_state s0.
 Proof.
   intros s H.
   core.Tactics.exploit_element_in_result H.
