transformations/Glue.v
@@ -1,4 +1,7 @@
 (** Generic type for Links *)
 
-Record Glue {A} {B} := { l_glue : A ; r_glue : B}.
+Record Glue A B := { l_glue : A ; r_glue : B}.
 Scheme Equality for Glue. (* Never used ? *)
+
+Arguments l_glue {A} {B}.
+Arguments r_glue {A} {B}.
